Cast optimization moved to Cminorgen. Updated Selection pass.
git-svn-id: https://yquem.inria.fr/compcert/svn/compcert/branches/nonstrict-ops@1775 fca1b0fc-160b-0410-b1d3-a4f43f01ea2e

cfrontend/Cminorgen.v
@@ -38,11 +38,9 @@ Local Open Scope error_monad_scope.
   taken in the Csharpminor code can be mapped to Cminor local
   variable, since the latter do not reside in memory.  
 
-  Another task performed during the translation to Cminor is the
-  insertion of truncation, zero- and sign-extension operations when
-  assigning to a Csharpminor local variable of ``small'' type
-  (e.g. [Mfloat32] or [Mint8signed]).  This is necessary to preserve
-  the ``normalize at assignment-time'' semantics of Clight and Csharpminor.
+  Another task performed during the translation to Cminor is to eliminate
+  redundant casts to small numerical types (8- and 16-bit integers,
+  single-precision floats).  
 
   Finally, the Clight-like [switch] construct of Csharpminor
   is transformed into the simpler, lower-level [switch] construct
@@ -77,7 +75,7 @@ Definition compilenv := PMap.t var_info.
 (** When the translation of an expression is stored in memory,
   one or several casts at the toplevel of the expression can be redundant
   with that implicitly performed by the memory store.
-  [uncast] detects this case and strips away the redundant casts. *)
+  [store_arg] detects this case and strips away the redundant cast. *)
 
 Function uncast_int8 (e: expr) : expr :=
   match e with
@@ -107,7 +105,7 @@ Function uncast_float32 (e: expr) : expr :=
   | _ => e
   end.
 
-Function uncast (chunk: memory_chunk) (e: expr) : expr :=
+Function store_arg (chunk: memory_chunk) (e: expr) : expr :=
   match chunk with
   | Mint8signed | Mint8unsigned => uncast_int8 e
   | Mint16signed | Mint16unsigned => uncast_int16 e
@@ -116,7 +114,7 @@ Function uncast (chunk: memory_chunk) (e: expr) : expr :=
   end.
 
 Definition make_store (chunk: memory_chunk) (e1 e2: expr): stmt :=
-  Sstore chunk e1 (uncast chunk e2).
+  Sstore chunk e1 (store_arg chunk e2).
 
 Definition make_stackaddr (ofs: Z): expr :=
   Econst (Oaddrstack (Int.repr ofs)).
@@ -124,16 +122,142 @@ Definition make_stackaddr (ofs: Z): expr :=
 Definition make_globaladdr (id: ident): expr :=
   Econst (Oaddrsymbol id Int.zero).
 
+Definition make_unop (op: unary_operation) (e: expr): expr :=
+  match op with
+  | Ocast8unsigned => Eunop Ocast8unsigned (uncast_int8 e)
+  | Ocast8signed => Eunop Ocast8signed (uncast_int8 e)
+  | Ocast16unsigned => Eunop Ocast16unsigned (uncast_int16 e)
+  | Ocast16signed => Eunop Ocast16signed (uncast_int16 e)
+  | Osingleoffloat => Eunop Osingleoffloat (uncast_float32 e)
+  | _ => Eunop op e
+  end.
+
+(** * Optimization of casts *)
+
+(** To remove redundant casts, we perform a modest static analysis
+  on the values of expressions, classifying them into the following
+  ranges. *)
+
+Inductive approx : Type :=
+  | Any                   (**r any value *)
+  | Int7                  (**r [[0,127]] *)
+  | Int8s                 (**r [[-128,127]] *)
+  | Int8u                 (**r [[0,255]] *)
+  | Int15                 (**r [[0,32767]] *)
+  | Int16s                (**r [[-32768,32767]] *)
+  | Int16u                (**r [[0,65535]] *)
+  | Float32.               (**r single-precision float *)
+
+Module Approx.
+
+Definition bge (x y: approx) : bool :=
+  match x, y with
+  | Any, _ => true
+  | Int7, Int7 => true
+  | Int8s, (Int7 | Int8s) => true
+  | Int8u, (Int7 | Int8u) => true
+  | Int15, (Int7 | Int8u | Int15) => true
+  | Int16s, (Int7 | Int8s | Int8u | Int15 | Int16s) => true
+  | Int16u, (Int7 | Int8u | Int15 | Int16u) => true
+  | Float32, Float32 => true
+  | _, _ => false
+  end.
+
+Definition lub (x y: approx) : approx :=
+  match x, y with
+  | Int7, Int7 => Int7
+  | Int7, Int8u => Int8u
+  | Int7, Int8s => Int8s
+  | Int7, Int15 => Int15
+  | Int7, Int16u => Int16u
+  | Int7, Int16s => Int16s
+  | Int8u, (Int7|Int8u) => Int8u
+  | Int8u, Int15 => Int15
+  | Int8u, Int16u => Int16u
+  | Int8u, Int16s => Int16s
+  | Int8s, (Int7|Int8s) => Int8s
+  | Int8s, (Int15|Int16s) => Int16s
+  | Int15, (Int7|Int8u|Int15) => Int15
+  | Int15, Int16u => Int16u
+  | Int15, (Int8s|Int16s) => Int16s
+  | Int16u, (Int7|Int8u|Int15|Int16u) => Int16u
+  | Int16s, (Int7|Int8u|Int8s|Int15|Int16s) => Int16s
+  | Float32, Float32 => Float32
+  | _, _ => Any
+  end.
+
+Definition of_int (n: int) :=
+  if Int.eq_dec n (Int.zero_ext 7 n) then Int7
+  else if Int.eq_dec n (Int.zero_ext 8 n) then Int8u
+  else if Int.eq_dec n (Int.sign_ext 8 n) then Int8s
+  else if Int.eq_dec n (Int.zero_ext 15 n) then Int15
+  else if Int.eq_dec n (Int.zero_ext 16 n) then Int16u
+  else if Int.eq_dec n (Int.sign_ext 16 n) then Int16s
+  else Any.
+
+Definition of_float (n: float) :=
+  if Float.eq_dec n (Float.singleoffloat n) then Float32 else Any.
+
+Definition of_chunk (chunk: memory_chunk) :=
+  match chunk with
+  | Mint8signed => Int8s
+  | Mint8unsigned => Int8u
+  | Mint16signed => Int16s
+  | Mint16unsigned => Int16u
+  | Mint32 => Any
+  | Mfloat32 => Float32
+  | Mfloat64 => Any
+  end.
+
+Definition unop (op: unary_operation) (a: approx) :=
+  match op with
+  | Ocast8unsigned => Int8u
+  | Ocast8signed => Int8s
+  | Ocast16unsigned => Int16u
+  | Ocast16signed => Int16s
+  | Osingleoffloat => Float32
+  | Onotbool => Int7
+  | _ => Any
+  end.
+
+Definition unop_is_redundant (op: unary_operation) (a: approx) :=
+  match op with
+  | Ocast8unsigned => bge Int8u a
+  | Ocast8signed => bge Int8s a
+  | Ocast16unsigned => bge Int16u a
+  | Ocast16signed => bge Int16s a
+  | Osingleoffloat => bge Float32 a
+  | _ => false
+  end.
+
+Definition bitwise_op (a1 a2: approx) :=
+  if bge Int8u a1 && bge Int8u a2 then Int8u
+  else if bge Int16u a1 && bge Int16u a2 then Int16u
+  else Any.
+
+Definition binop (op: binary_operation) (a1 a2: approx) :=
+  match op with
+  | Oand | Oor | Oxor => bitwise_op a1 a2
+  | Ocmp _ => Int7
+  | Ocmpu _ => Int7
+  | Ocmpf _ => Int7
+  | _ => Any
+  end.
+
+End Approx.
+
 (** * Translation of expressions and statements. *)
 
-Definition var_get (cenv: compilenv) (id: ident): res expr :=
+(** Generation of a Cminor expression for reading a Csharpminor variable. *)
+
+Definition var_get (cenv: compilenv) (id: ident): res (expr * approx) :=
   match PMap.get id cenv with
   | Var_local chunk =>
-      OK(Evar (for_var id))
+      OK(Evar (for_var id), Approx.of_chunk chunk)
   | Var_stack_scalar chunk ofs =>
-      OK(Eload chunk (make_stackaddr ofs))
+      OK(Eload chunk (make_stackaddr ofs), Approx.of_chunk chunk)
   | Var_global_scalar chunk =>
-      OK(Eload chunk (make_globaladdr id))
+      OK(Eload chunk (make_globaladdr id), Approx.of_chunk chunk)
   | _ =>
       Error(msg "Cminorgen.var_get")
   end.
@@ -141,12 +265,12 @@ Definition var_get (cenv: compilenv) (id: ident): res expr :=
 (** Generation of a Cminor expression for taking the address of
   a Csharpminor variable. *)
 
-Definition var_addr (cenv: compilenv) (id: ident): res expr :=
+Definition var_addr (cenv: compilenv) (id: ident): res (expr * approx) :=
   match PMap.get id cenv with
   | Var_local chunk => Error(msg "Cminorgen.var_addr")
-  | Var_stack_scalar chunk ofs => OK (make_stackaddr ofs)
-  | Var_stack_array ofs => OK (make_stackaddr ofs)
-  | _ => OK (make_globaladdr id)
+  | Var_stack_scalar chunk ofs => OK (make_stackaddr ofs, Any)
+  | Var_stack_array ofs => OK (make_stackaddr ofs, Any)
+  | _ => OK (make_globaladdr id, Any)
   end.
 
 (** Generation of a Cminor statement performing an assignment to
@@ -183,38 +307,46 @@ Definition var_set_self (cenv: compilenv) (id: ident) (ty: typ) (k: stmt): res s
 
 (** Translation of constants. *)
 
-Definition transl_constant (cst: Csharpminor.constant): constant :=
+Definition transl_constant (cst: Csharpminor.constant): (constant * approx) :=
   match cst with
-  | Csharpminor.Ointconst n => Ointconst n
-  | Csharpminor.Ofloatconst n => Ofloatconst n
+  | Csharpminor.Ointconst n =>
+      (Ointconst n, Approx.of_int n)
+  | Csharpminor.Ofloatconst n =>
+      (Ofloatconst n, Approx.of_float n)
   end.
 
-(** Translation of expressions.  All the hard work is done by the
-  [make_*] and [var_*] functions defined above. *)
+(** Translation of expressions.  Return both a Cminor expression and
+  a compile-time approximation of the value of the original
+  C#minor expression, which is used to remove redundant casts. *)
 
 Fixpoint transl_expr (cenv: compilenv) (e: Csharpminor.expr)
-                     {struct e}: res expr :=
+                     {struct e}: res (expr * approx) :=
   match e with
-  | Csharpminor.Evar id => var_get cenv id
-  | Csharpminor.Etempvar id => OK (Evar (for_temp id))
-  | Csharpminor.Eaddrof id => var_addr cenv id
+  | Csharpminor.Evar id =>
+      var_get cenv id
+  | Csharpminor.Etempvar id =>
+      OK (Evar (for_temp id), Any)
+  | Csharpminor.Eaddrof id =>
+      var_addr cenv id
   | Csharpminor.Econst cst =>
-      OK (Econst (transl_constant cst))
+      let (tcst, a) := transl_constant cst in OK (Econst tcst, a)
   | Csharpminor.Eunop op e1 =>
-      do te1 <- transl_expr cenv e1;
-      OK (Eunop op te1)
+      do (te1, a1)  <- transl_expr cenv e1;
+      if Approx.unop_is_redundant op a1
+      then OK (te1, a1)
+      else OK (make_unop op te1, Approx.unop op a1)
   | Csharpminor.Ebinop op e1 e2 =>
-      do te1 <- transl_expr cenv e1;
-      do te2 <- transl_expr cenv e2;
-      OK (Ebinop op te1 te2)
+      do (te1, a1) <- transl_expr cenv e1;
+      do (te2, a2) <- transl_expr cenv e2;
+      OK (Ebinop op te1 te2, Approx.binop op a1 a2)
   | Csharpminor.Eload chunk e =>
-      do te <- transl_expr cenv e;
-      OK (Eload chunk te)
+      do (te, a) <- transl_expr cenv e;
+      OK (Eload chunk te, Approx.of_chunk chunk)
   | Csharpminor.Econdition e1 e2 e3 =>
-      do te1 <- transl_expr cenv e1;
-      do te2 <- transl_expr cenv e2;
-      do te3 <- transl_expr cenv e3;
-      OK (Econdition te1 te2 te3)
+      do (te1, a1) <- transl_expr cenv e1;
+      do (te2, a2) <- transl_expr cenv e2;
+      do (te3, a3) <- transl_expr cenv e3;
+      OK (Econdition te1 te2 te3, Approx.lub a2 a3)
   end.
 
 Fixpoint transl_exprlist (cenv: compilenv) (el: list Csharpminor.expr)
@@ -223,7 +355,7 @@ Fixpoint transl_exprlist (cenv: compilenv) (el: list Csharpminor.expr)
   | nil =>
       OK nil
   | e1 :: e2 =>
-      do te1 <- transl_expr cenv e1;
+      do (te1, a1) <- transl_expr cenv e1;
       do te2 <- transl_exprlist cenv e2;
       OK (te1 :: te2)
   end.
@@ -269,12 +401,7 @@ Fixpoint switch_env (ls: lbl_stmt) (e: exit_env) {struct ls}: exit_env :=
   end.
 
 (** Translation of statements.  The nonobvious part is
-  the translation of [switch] statements, outlined above. 
-  Also note the additional type checks on arguments to calls and returns.
-  These checks should always succeed for C#minor code generated from
-  well-typed Clight code, but are necessary for the correctness proof
-  to go through.
-*)
+  the translation of [switch] statements, outlined above. *)
 
 Definition typ_of_opttyp (ot: option typ) :=
   match ot with None => Tint | Some t => t end.
@@ -286,17 +413,17 @@ Fixpoint transl_stmt (ret: option typ) (cenv: compilenv)
   | Csharpminor.Sskip =>
       OK Sskip
   | Csharpminor.Sassign id e =>
-      do te <- transl_expr cenv e;
+      do (te, a) <- transl_expr cenv e;
       var_set cenv id te
   | Csharpminor.Sset id e =>
-      do te <- transl_expr cenv e;
+      do (te, a) <- transl_expr cenv e;
       OK (Sassign (for_temp id) te)
   | Csharpminor.Sstore chunk e1 e2 =>
-      do te1 <- transl_expr cenv e1;
-      do te2 <- transl_expr cenv e2;
+      do (te1, a1) <- transl_expr cenv e1;
+      do (te2, a2) <- transl_expr cenv e2;
       OK (make_store chunk te1 te2)
   | Csharpminor.Scall optid sig e el =>
-      do te <- transl_expr cenv e;
+      do (te, a) <- transl_expr cenv e;
       do tel <- transl_exprlist cenv el;
       OK (Scall (option_map for_temp optid) sig te tel)
   | Csharpminor.Sseq s1 s2 =>
@@ -304,7 +431,7 @@ Fixpoint transl_stmt (ret: option typ) (cenv: compilenv)
       do ts2 <- transl_stmt ret cenv xenv s2;
       OK (Sseq ts1 ts2)
   | Csharpminor.Sifthenelse e s1 s2 =>
-      do te <- transl_expr cenv e;
+      do (te, a) <- transl_expr cenv e;
       do ts1 <- transl_stmt ret cenv xenv s1;
       do ts2 <- transl_stmt ret cenv xenv s2;
       OK (Sifthenelse te ts1 ts2)
@@ -319,12 +446,12 @@ Fixpoint transl_stmt (ret: option typ) (cenv: compilenv)
   | Csharpminor.Sswitch e ls =>
       let cases := switch_table ls O in
       let default := length cases in
-      do te <- transl_expr cenv e;
+      do (te, a) <- transl_expr cenv e;
       transl_lblstmt ret cenv (switch_env ls xenv) ls (Sswitch te cases default)
   | Csharpminor.Sreturn None =>
       OK (Sreturn None)
   | Csharpminor.Sreturn (Some e) =>
-      do te <- transl_expr cenv e;
+      do (te, a) <- transl_expr cenv e;
       OK (Sreturn (Some te))
   | Csharpminor.Slabel lbl s =>
       do ts <- transl_stmt ret cenv xenv s; OK (Slabel lbl ts)
